Heaps.thy
@@ -1,0 +1,147 @@
+(* @LICENSE(NICTA_CORE) *)
+
+(*  Author:     Rafal Kolanski, NICTA & UNSW 
+
+    Generic heap definitions and manipulations instantiated to a machine.
+*)
+
+theory Heaps
+imports MemTypes WordTypes
+begin
+
+section {* Memory Views *}
+
+text {*
+  Apart from the heap, representing the physical machine memory, we recognise
+  the virtual address map (mapping each virtual address to a physical one) and
+  the virtual address space (mapping each virtual address to a byte).
+  
+  You can obtain a virtual map from lifting the page table from the heap, and
+  an address space from combining a vmap and heap.
+  
+  All maps are partial. On the physical side, this denotes memory that has been
+  allocated. On the virtual side, memory that has been mapped. Allocated memory
+  may be unmapped, mapped memory may be unallocated.
+  
+  The heap is partial, defined on areas used by the program.
+
+  A value space is a partial map from any kind of address to bytes.
+  *}
+type_synonym vmap = "vaddr \<rightharpoonup> paddr"
+type_synonym heap = "paddr \<rightharpoonup> byte"
+type_synonym addr_space = "vaddr \<rightharpoonup> byte"
+
+translations
+  (type) "vmap" <=(type) "vaddr \<rightharpoonup> paddr"
+  (type) "heap" <=(type) "paddr \<rightharpoonup> byte"
+  (type) "addr_space" <=(type) "vaddr \<rightharpoonup> byte"
+
+type_synonym ('a,'p) value_space = "('a,'p) addr_t \<rightharpoonup> byte"
+
+
+section {* Object Loading *}
+
+text {* Obtaining a list of values (i.e. bytes) from a map with an addr_t domain. *}
+
+primrec
+  load_list_basic :: "(('a::semiring_1,'p) addr_t \<rightharpoonup> 'val) \<Rightarrow> nat 
+                      \<Rightarrow> ('a,'p) addr_t \<Rightarrow> 'val option list"
+where
+  "load_list_basic h 0 p = []" |
+  "load_list_basic h (Suc n) p = h p # load_list_basic h n (p r+ 1)"
+
+definition
+  deoption_list :: "'a option list \<rightharpoonup> 'a list" where
+  "deoption_list xs \<equiv> if None \<in> set xs then None else Some (map the xs)"
+
+definition
+  "load_list h n p \<equiv> deoption_list (load_list_basic h n p)"
+
+lemma length_load_list_basic [simp]:
+  "length (load_list_basic h sz p) = sz"
+  by (induct sz arbitrary: p, auto)
+
+
+section {* Loading Objects from the Heap/Address Space *}
+
+text {* Retrieving a stored value on the heap or addr\_space *}
+(* FIXME: ugly return-type overloading, improve? *)
+
+definition
+  load_value :: "('a::semiring_1,'p) value_space \<Rightarrow> ('a,'p) addr_t 
+                  \<rightharpoonup> ('t::mem_type)" where
+  "load_value h p \<equiv> (case load_list h (size_of TYPE('t)) p 
+                       of None \<Rightarrow> None
+                        | Some bs \<Rightarrow> Some (from_bytes bs))"
+
+(* update form Hira: changed Option.map to map_option *)
+lemma load_value_def2:
+  "((load_value h p)::'t option) \<equiv> map_option from_bytes (load_list h (size_of TYPE('t::mem_type)) p)"
+  by (auto intro!: eq_reflection simp: load_value_def split: option.splits)
+
+definition
+  load_machine_word :: "('a::semiring_1,'p) value_space \<Rightarrow> ('a,'p) addr_t 
+                        \<rightharpoonup> machine_word" where
+  "load_machine_word \<equiv> load_value"
+
+subsection {* Loading Objects After Unrelated Heap Updates *}
+
+lemma load_list_basic_update_eq:
+  assumes p: "p \<notin> set (addr_seq start sz)"
+  shows "load_list_basic (h(p \<mapsto> v)) sz start = load_list_basic h sz start"
+  using p proof (induct sz arbitrary: start)
+  case 0 thus ?case by simp
+next
+  case (Suc sz start)
+  hence IH: "p \<notin> set (addr_seq (start r+ 1) sz)
+             \<Longrightarrow> load_list_basic (h(p \<mapsto> v)) sz (start r+ 1) = 
+                 load_list_basic h sz (start r+ 1)"
+    and ps: "p \<notin> set (addr_seq start (Suc sz))" by - assumption
+  (*WTF:blast or simp don't work here? why?*)
+
+  from ps have "p \<notin> set (addr_seq (start r+ 1) sz)" by auto
+
+  hence "load_list_basic (h(p \<mapsto> v)) sz (start r+ 1) = 
+           load_list_basic h sz (start r+ 1)" using IH by simp
+
+  moreover 
+
+  have "(\<lambda>a. if a = p then Some v else h a) = h(p \<mapsto> v)"
+    by (rule ext, auto)
+
+  moreover
+
+  have "p \<noteq> start" using ps
+    proof -
+      assume "start = p"
+      hence "p \<in> set (addr_seq start (Suc sz))" by simp
+    qed (auto)
+
+  ultimately show ?case by (clarsimp)
+qed
+
+lemma load_list_update_eq:
+  "\<lbrakk> p \<notin> set (addr_seq start sz) \<rbrakk>
+   \<Longrightarrow> load_list (h(p \<mapsto> v)) sz start = load_list h sz start"
+  unfolding load_list_def deoption_list_def 
+  by (simp add: load_list_basic_update_eq)
+
+lemma load_value_update_eq:
+  "\<lbrakk> p \<notin> set (addr_seq start (size_of TYPE('a::mem_type))) \<rbrakk>
+   \<Longrightarrow> load_value (h(p \<mapsto> v)) start = ((load_value h start)::'a option)"
+  unfolding load_machine_word_def load_value_def Let_def
+  by (simp add: load_list_update_eq)
+
+lemma load_list_basic_nth [simp]:
+  fixes p :: "('a::len word,'b) addr_t"
+  shows "i < sz \<Longrightarrow> load_list_basic h sz p ! i = h (p r+ (of_nat i))"
+proof (induct sz arbitrary: p i)
+  case 0 thus ?case by simp
+next
+  case (Suc sz)
+  thus ?case
+  by (clarsimp simp: nth_Cons')
+     (cases i, auto simp add: addr_add_def add_ac split: nat.split)
+qed
+
+end
