WordsARM.thy
@@ -1,0 +1,49 @@
+(* @LICENSE(NICTA_CORE) *)
+
+theory WordsARM
+imports "~~/src/HOL/Word/Word"
+begin
+
+class word_len_1 = len +
+  assumes word_len_1: "len_of TYPE('a) = 1"
+
+class word_len_1_2 = len +
+  assumes word_len_1_2: "len_of TYPE('a) = 1 \<or> len_of TYPE('a) = 2"
+
+class word_len_1_2_4 = len + 
+  assumes word_len_1_2_4: "len_of TYPE('a) = 1 \<or> len_of TYPE('a) = 2 \<or> len_of TYPE('a) = 4"
+
+class word_len_2_4_8 = len + 
+  assumes word_len_2_4_8: "len_of TYPE('a) = 2 \<or> len_of TYPE('a) = 4 \<or> len_of TYPE('a) = 8"
+
+class word_len_4_8_16 = len + 
+  assumes word_len_4_8_16: "len_of TYPE('a) = 4 \<or> len_of TYPE('a) = 8 \<or> len_of TYPE('a) = 16"
+
+class word_len_8_16_32 = len + 
+  assumes word_len_8_16_32: "len_of TYPE('a) = 8 \<or> len_of TYPE('a) = 16 \<or> len_of TYPE('a) = 32"
+
+instance num1 :: word_len_1
+  by (intro_classes, simp)
+
+instance num1 :: word_len_1_2
+  by (intro_classes, simp)
+
+instance num1 :: word_len_1_2_4
+  by (intro_classes, simp)
+
+instance bit0 :: (word_len_1) word_len_1_2
+  by (intro_classes, simp add: word_len_1)
+
+instance bit0 :: (word_len_1_2) word_len_1_2_4
+  by (intro_classes, insert word_len_1_2, simp)
+
+instance bit0 :: (word_len_1_2_4) word_len_2_4_8
+  by (intro_classes, insert word_len_1_2_4, simp)
+
+instance bit0 :: (word_len_2_4_8) word_len_4_8_16
+  by (intro_classes, insert word_len_2_4_8, simp)
+
+instance bit0 :: (word_len_4_8_16) word_len_8_16_32
+  by (intro_classes, insert word_len_4_8_16, simp)
+
+end
