reduntant.thy
@@ -1,0 +1,887 @@
+
+
+
+
+
+
+
+
+
+
+
+
+
+(*
+
+lemma
+  "\<lbrakk>write'mem1 (val, HOL.undefined , sz) (b\<lparr>exception := PAGE_FAULT ''more info''\<rparr>)  = ((), ba) \<rbrakk>  
+       \<Longrightarrow>  exception ba = PAGE_FAULT ''more info''"
+  by (clarsimp simp: write'mem1_def raise'exception_def split:split_if_asm)
+
+
+lemma
+  "\<lbrakk> mem1s (va, sz) (ba\<lparr>TLB := TLB ba \<union> range (pt_walk (ASID ba) (MEM ba) (TTBR0 ba))\<rparr>) = (val, r) ;
+       exception ba = PAGE_FAULT ''more info'' \<rbrakk>   \<Longrightarrow> exception r = PAGE_FAULT ''more info''"
+  apply (clarsimp simp: mem1s_def)
+  apply (cases " mmu_translate_sat va (ba\<lparr>TLB := TLB ba \<union> range (pt_walk (ASID ba) (MEM ba) (TTBR0 ba))\<rparr>)" , clarsimp)
+  (* first reason about exception of b *)
+  apply (clarsimp simp: mmu_translate_sat_def Let_def)
+  apply (cases "lookup (TLB ba \<union> range (pt_walk (ASID ba) (MEM ba) (TTBR0 ba))) (ASID ba) (addr_val va) ")
+    prefer 3
+    apply (clarsimp)
+   apply (clarsimp simp: mem_def split:split_if_asm)
+    apply (case_tac "mem1 (a r+ 0) b" , clarsimp)
+    apply (clarsimp split: split_if_asm)
+     apply (clarsimp simp: raise'exception_def split: split_if_asm)  
+
+
+oops
+
+lemma state:
+  "\<lbrakk> write'mem'sat' (val,va,sz) s = ((), t); mem1s (va, sz) t = (val, r); consistent t va \<rbrakk> 
+                       \<Longrightarrow> t = r"
+  apply (clarsimp simp: write'mem'sat'_def)
+  apply (cases "mmu_translate_sat va s" , clarsimp)
+  apply (clarsimp simp: mmu_translate_sat_def Let_def)
+  apply (cases "lookup (TLB s \<union> range (pt_walk (ASID s) (MEM s) (TTBR0 s))) (ASID s) (addr_val va)")
+    apply (clarsimp simp: saturated_not_miss)
+   apply (subgoal_tac "TLB s \<union> range (pt_walk (ASID s) (MEM s) (TTBR0 s)) = TLB t \<and> ASID s = ASID t")
+    apply (clarsimp simp: consistent0_def)
+   apply (case_tac "write'mem1 (val, a, sz) b" , clarsimp)
+    apply (subgoal_tac "lookup (TLB s) (ASID s) (addr_val va) \<le> lookup (TLB s \<union> range (pt_walk (ASID s) (MEM s) (TTBR0 s))) (ASID s) (addr_val va)")
+     prefer 2
+     apply (simp add: tlb_mono)
+
+    apply (clarsimp simp: consistent0_def)
+   
+   apply (clarsimp simp: write'mem'sat'_def)
+   apply (cases "mmu_translate_sat va s" , clarsimp)
+   apply (clarsimp simp: mmu_translate_sat_def Let_def)
+   apply (cases "lookup (TLB s \<union> range (pt_walk (ASID s) (MEM s) (TTBR0 s))) (ASID s) (addr_val va)")
+     apply (clarsimp simp: saturated_not_miss)
+   apply (case_tac "write'mem1 (val, a, sz) b " , clarsimp)
+   apply (subgoal_tac "consistent b va")
+    apply (clarsimp simp: mmu_translate_sat_def Let_def)
+    apply (cases "lookup (TLB s \<union> range (pt_walk (ASID s) (MEM s) (TTBR0 s))) (ASID s) (addr_val va)")
+      apply (clarsimp simp: saturated_not_miss)
+     apply (subgoal_tac "TLB s \<union> range (pt_walk (ASID s) (MEM s) (TTBR0 s)) = TLB b \<and>
+                           ASID s = ASID b")
+      apply (clarsimp simp: consistent0_def)
+     apply (clarsimp simp: raise'exception_def split:split_if_asm)
+    apply clarsimp
+    apply (case_tac "is_fault x3")
+     apply (clarsimp)
+     apply (subgoal_tac "exception ba = PAGE_FAULT ''more info''")
+      apply (clarsimp)
+
+
+
+    apply (clarsimp split: split_if_asm)
+     apply (clarsimp simp: raise'exception_def split: split_if_asm)
+      
+     
+
+
+oops
+ mem1s_def mmu_translate_sat_def Let_def split:prod.splits)
+  apply (cases "lookup (TLB s \<union> range (pt_walk (ASID s) (MEM s) (TTBR0 s))) (ASID s) (addr_val va)")
+    apply (clarsimp simp: saturated_not_miss)
+   apply (subgoal_tac "TLB t = TLB s \<union> range (pt_walk (ASID s) (MEM s) (TTBR0 s))")
+    apply (subgoal_tac "MEM x2b = MEM s \<and> ASID x2b = ASID s \<and> TTBR0 x2b = TTBR0 s \<and> TLB x2b = TLB s")
+     apply (clarsimp simp: consistent0_def)
+  apply (clarsimp simp: write'mem1_def)
+  apply (clarsimp split: split_if_asm)
+      apply (clarsimp simp: Let_def)
+      apply (clarsimp simp: mem1s_def split: prod.splits)
+      apply (clarsimp simp: mem_def split: prod.splits)
+      apply (clarsimp split: split_if_asm)
+         apply (clarsimp simp: raise'exception_def split:split_if_asm)
+
+
+  
+oops
+lemma same_state:
+  "\<lbrakk>mem1s (va, sz) t = (val, r) ; TLB t = TLB r; MEM t = MEM r \<rbrakk>  
+      \<Longrightarrow> exception t = exception r"
+  apply (clarsimp simp: mem1s_def split:prod.splits)
+  apply (subgoal_tac "TLB t = TLB x2 \<and> MEM t = MEM x2 ")
+   apply (subgoal_tac "exception t = exception x2")
+    prefer 2
+    apply (clarsimp simp: mmu_translate_sat_def Let_def split:prod.splits)
+    apply (cases "lookup (TLB r \<union> range (pt_walk (ASID t) (MEM r) (TTBR0 t))) (ASID t) (addr_val va)")
+    prefer 3
+    apply (clarsimp simp: raise'exception_def split:split_if_asm)
+oops
+
+(*lemma
+  "\<lbrakk> write'mem'det (val,va, sz) s = ((), s'); consistent t va; tlb_rel_sat s t ;
+        write'mem'sat' (val,va, sz) t = ((), t') \<rbrakk> \<Longrightarrow> tlb_rel_sat s' t'"
+  apply (clarsimp simp: tlb_rel_sat_def)
+  apply (clarsimp simp:  write'_not_in_translation_tables_saturated)
+  apply (rule conjI)
+  prefer 2
+  apply (frule_tac s="s" and s'="s'" and t="t" and t'="t'" in tlb_rel_1; clarsimp simp: tlb_rel_sat_def)
+   apply (frule_tac s="s" and s'="s'" and t="t" and t'="t'" in tlb_rel_2; clarsimp simp: tlb_rel_sat_def)
+  done
+  *)
+
+
+(*lemma inter:
+  "\<lbrakk> mem1 pa s = (val, t) \<rbrakk>  \<Longrightarrow> t = s \<lparr>exception:= exception t\<rparr>"
+  apply (clarsimp simp: mem1_def raise'exception_def split:option.splits split_if_asm)
+done
+
+lemma inter1:
+  "\<lbrakk> mem1 pa s = (val, t) \<rbrakk>  \<Longrightarrow> TLB t = TLB s"
+  apply (clarsimp simp: mem1_def raise'exception_def split:option.splits split_if_asm)
+done
+
+lemma inter2:
+  "\<lbrakk> mem1 pa s = (val, t) \<rbrakk>  \<Longrightarrow> TLB (snd(mem1 pa s)) = TLB t"
+  apply (clarsimp simp: mem1_def raise'exception_def split:option.splits split_if_asm)
+done
+
+lemma mem1_rewrite:
+  "snd (mem1 p s) = s \<lparr>exception:= exception (snd (mem1 p s) ) \<rparr>"
+  apply (clarsimp simp: mem1_def raise'exception_def split:option.splits split_if_asm)
+  done
+
+lemma mem1_rewrite_excpetion:
+  "snd (mem1 p s)\<lparr>exception := UNPREDICTABLE ''undefined memory''\<rparr> = s
+              \<lparr>exception := UNPREDICTABLE ''undefined memory''\<rparr>"
+apply (clarsimp simp: mem1_def raise'exception_def split:option.splits split_if_asm)
+  done
+
+lemma aa:
+  "mem (pa, 1) s = (val, t) \<Longrightarrow> t = s\<lparr>exception:= exception t\<rparr>"
+  apply (subgoal_tac "\<forall>p s. snd (mem1 p s) = s \<lparr>exception:= exception (snd (mem1 p s))\<rparr>")
+   apply (subgoal_tac "\<forall>p s. snd (mem1 p s) \<lparr>exception := UNPREDICTABLE ''undefined memory''\<rparr>  =
+            s \<lparr>exception := UNPREDICTABLE ''undefined memory''\<rparr>")
+    apply (clarsimp simp: mem_def split_def Let_def split: split_if_asm)
+    apply (clarsimp simp: raise'exception_def split:split_if_asm)
+   apply (clarsimp simp: mem1_def raise'exception_def split:option.splits split_if_asm)
+  apply (clarsimp simp: mem1_def raise'exception_def split:option.splits split_if_asm)
+done
+    
+   
+
+
+
+lemma aa1:
+  "mem (pa, 2) s = (val, t) \<Longrightarrow> t = s\<lparr>exception:= exception t\<rparr>"
+  apply (subgoal_tac "\<forall>p s. snd (mem1 p s) = s \<lparr>exception:= exception (snd (mem1 p s))\<rparr>")
+   apply (subgoal_tac "\<forall>p s. snd (mem1 p s) \<lparr>exception := UNPREDICTABLE ''undefined memory''\<rparr>  =
+            s \<lparr>exception := UNPREDICTABLE ''undefined memory''\<rparr>")
+     apply (clarsimp simp: mem_def split_def Let_def split: split_if_asm)
+        apply (clarsimp simp: raise'exception_def split:split_if_asm)
+       apply (clarsimp simp: raise'exception_def split:split_if_asm)
+       apply (clarsimp simp: mem1_def raise'exception_def split:option.splits split_if_asm)
+      apply (clarsimp simp: mem1_def raise'exception_def split:option.splits split_if_asm)
+     apply (clarsimp simp: raise'exception_def split:split_if_asm)
+    apply (clarsimp simp: mem1_def raise'exception_def split:option.splits split_if_asm)
+   apply (clarsimp simp: mem1_def raise'exception_def split:option.splits split_if_asm)
+  apply (clarsimp simp: mem1_def raise'exception_def split:option.splits split_if_asm)
+  apply (clarsimp simp: mem1_def raise'exception_def split:option.splits split_if_asm)
+done
+  
+lemma aa2:
+  "mem (pa, sz) s = (val, t) \<Longrightarrow> t = s\<lparr>exception:= exception t\<rparr>"
+  apply (subgoal_tac "\<forall>p s. snd (mem1 p s) = s \<lparr>exception:= exception (snd (mem1 p s))\<rparr>")
+   apply (subgoal_tac "\<forall>p s. snd (mem1 p s) \<lparr>exception := UNPREDICTABLE ''undefined memory''\<rparr>  =
+            s \<lparr>exception := UNPREDICTABLE ''undefined memory''\<rparr>")
+    apply (clarsimp simp: mem_def split_def Let_def) 
+    apply (clarsimp split: split_if_asm)
+        apply (clarsimp simp: split_def Let_def raise'exception_def split:split_if_asm)
+       apply (clarsimp simp: split_def Let_def raise'exception_def split:split_if_asm)
+          apply (clarsimp simp: mem1_def raise'exception_def split:option.splits split_if_asm)
+         apply (clarsimp simp: mem1_def raise'exception_def split:option.splits split_if_asm)
+        apply (clarsimp simp: mem1_def raise'exception_def split:option.splits split_if_asm)
+       apply (clarsimp simp: mem1_def raise'exception_def split:option.splits split_if_asm)
+      apply (clarsimp simp: split_def Let_def raise'exception_def split:split_if_asm)
+             apply (clarsimp simp: mem1_def raise'exception_def)
+             apply (clarsimp split:option.splits split_if_asm)
+             apply (clarsimp simp: raise'exception_def)
+               apply (clarsimp simp: raise'exception_def)
+        apply (clarsimp simp: mem1_def raise'exception_def)
+             apply (clarsimp split:option.splits split_if_asm)
+
+          apply (fastforce simp: raise'exception_def)
+           apply (auto simp: raise'exception_def) [1]     
+            apply (auto simp: raise'exception_def) [1]  
+        apply (auto simp: raise'exception_def) [1]  
+                apply (auto simp: raise'exception_def) [1]   
+        apply (clarsimp simp: mem1_def raise'exception_def)
+             apply (clarsimp simp: mem1_def raise'exception_def)
+      apply (clarsimp split:option.splits split_if_asm)
+     apply (auto simp: raise'exception_def) [1] 
+    apply (auto simp: raise'exception_def) [1]
+      apply (auto simp: raise'exception_def) [1]  
+apply (auto simp: raise'exception_def) [9]  
+apply (auto simp: raise'exception_def) [2]  
+ apply (clarsimp simp: mem1_def raise'exception_def)
+     
+       
+oops
+
+
+
+
+lemma a:
+  "mem (pa, sz) s = (val, t) \<Longrightarrow> TLB s = TLB t"
+  apply (cases s , cases t)
+  apply (drule aa)
+  apply (clarsimp simp: aa)
+  done
+
+lemma b:
+  "\<lbrakk> mem1s (va, sz) s = (val, t) ; saturated s \<rbrakk>  \<Longrightarrow> TLB t = TLB s"
+  apply (clarsimp simp: mem1s_def split_def Let_def)
+  apply (subgoal_tac "TLB (snd (mmu_translate_sat va s)) = TLB s")
+   apply (subgoal_tac "TLB (snd (mem (fst (mmu_translate_sat va s), sz) (snd (mmu_translate_sat va s)))) =
+    TLB s")
+    apply clarsimp
+   prefer 2
+   apply (subgoal_tac "TLB (snd (mmu_translate_sat va s)) = TLB s \<union> pt_walk (ASID s) (MEM s) (TTBR0 s) ` UNIV")
+    apply (clarsimp simp: saturated_def)
+    apply blast
+   apply (clarsimp simp: mmu_translate_sat_def Let_def split_def)
+   apply (cases "lookup (TLB s \<union> range (pt_walk (ASID s) (MEM s) (TTBR0 s))) (ASID s) (addr_val va)"; clarsimp simp: raise'exception_def)
+  apply clarsimp
+  apply (subgoal_tac "TLB t = TLB (snd (mmu_translate_sat va s))")
+   apply clarsimp
+  apply (clarsimp simp: a)
+  done
+  
+
+lemma write'_not_in_translation_tables_TLB:
+  "\<lbrakk> write'mem'sat' (val,va,sz) s = ((), t); mem1s (va, sz) t = (val, r) \<rbrakk> 
+        \<Longrightarrow> (TLB t) = (TLB r)"
+  apply (cases "\<not> ptable_trace (MEM s) (TTBR0 s) va \<subseteq> \<Union>(ptable_trace (MEM s) (TTBR0 s) ` UNIV)" )
+   apply (subgoal_tac "saturated t")
+    prefer 2
+    apply (clarsimp simp: write'_not_in_translation_tables_saturated)
+   apply (clarsimp simp: mem1s_def)
+   apply (cases "mmu_translate_sat va t" , clarsimp)
+   apply (clarsimp simp: mmu_translate_sat_def Let_def)
+   apply (cases
+     "lookup (TLB t \<union> range (pt_walk (ASID t) (MEM t) (TTBR0 t))) (ASID t) (addr_val va)")
+     apply (simp only: split_if_asm raise'exception_def saturated_def, force) +
+  apply simp
+  apply (subgoal_tac "saturated t")
+   prefer 2
+   apply (clarsimp simp: write'_not_in_translation_tables_saturated)
+  apply (clarsimp simp: b)
+done
+
+*)
+
+
+
+definition
+  mem1s1 :: "vaddr \<times> nat \<Rightarrow> state \<Rightarrow> bool list \<times> state"
+where
+  "mem1s1 \<equiv> \<lambda>(va, sz). do {
+                     pa  \<leftarrow> mmu_translate_sat va; 
+                     if pa = HOL.undefined 
+                     then return (HOL.undefined) 
+                     else (mem (pa, sz))
+  }"                           
+
+
+definition
+  "write'mem'sat'1" :: "bool list \<times> vaddr \<times> nat \<Rightarrow> state \<Rightarrow> unit \<times> state"
+where
+  "write'mem'sat'1 \<equiv> \<lambda>(value, va, size). do {
+     mem   <- read_state MEM;
+     ttbr0 <- read_state TTBR0;
+     asid <- read_state ASID;
+     (* original TLB before memory translation *)
+     pa <- mmu_translate_sat va;
+     if pa = HOL.undefined 
+      then return (HOL.undefined) 
+      else do { 
+           write'mem1 (value, pa, size); 
+           tlb0  <- read_state TLB;
+           mem1  <- read_state MEM;
+           let all_entries = pt_walk asid mem1 ttbr0 ` UNIV;
+           let tlb = tlb0 \<union> all_entries;  (* what about inconsistency here ? *)
+           update_state (\<lambda>s. s\<lparr> TLB := tlb \<rparr>)
+          } 
+    }"
+
+
+lemma write'_not_in_translation_tables_saturated1:
+  "\<lbrakk> write'mem'sat'1 (val,va,sz) s = ((), t)  \<rbrakk>  \<Longrightarrow> saturated t"
+  apply (clarsimp simp: write'mem'sat'1_def split_def Let_def)
+  apply (clarsimp split: split_if_asm)
+   apply (clarsimp simp: mmu_translate_sat_sat)
+  apply (clarsimp simp: split_def)
+  apply (subgoal_tac "ASID s = ASID (snd (write'mem1 (val, fst (mmu_translate_sat va s), sz) (snd (mmu_translate_sat va s)))) \<and>
+                       TTBR0 s = TTBR0 (snd (write'mem1 (val, fst (mmu_translate_sat va s), sz) (snd (mmu_translate_sat va s)))) ")
+   apply (clarsimp simp: saturated_def)
+  apply (subgoal_tac "ASID s = ASID (snd(mmu_translate_sat va s)) \<and> TTBR0 s = TTBR0 (snd(mmu_translate_sat va s))")
+   apply (clarsimp simp:  write'mem1_def Let_def raise'exception_def)
+  apply (clarsimp simp: mmu_translate_sat_def Let_def raise'exception_def split:lookup_type.splits)
+  done 
+
+
+(* see write'mem'det_TLBs *)
+lemma write'mem'sat'1_TLBs:
+  "\<lbrakk>write'mem'sat'1 (val,va, sz) s = ((), s') \<rbrakk> \<Longrightarrow>
+     TLB s' = TLB s \<union> range (pt_walk (ASID s) (MEM s) (TTBR0 s)) \<or>
+     TLB s' = TLB s \<union> range (pt_walk (ASID s) (MEM s) (TTBR0 s)) \<union> range (pt_walk (ASID s') (MEM s') (TTBR0 s'))"
+  apply (cases "fst (mmu_translate_sat va s) = HOL.undefined")
+   apply (simp only: write'mem'sat'1_def Let_def split_def)
+   apply (rule disjI1)
+   apply (clarsimp simp: split_def)
+   apply (metis mmu_translate_sat_TLB_union prod.collapse)
+  apply (clarsimp simp: write'mem'sat'1_def Let_def split_def)
+  apply (subgoal_tac "TLB (snd (write'mem1 (val, fst (mmu_translate_sat va s), sz) (snd (mmu_translate_sat va s)))) = TLB (snd (mmu_translate_sat va s))")
+   apply clarsimp
+   apply (subgoal_tac "TLB (snd (mmu_translate_sat va s)) = TLB s \<union> range (pt_walk (ASID s) (MEM s) (TTBR0 s))")
+    apply (subgoal_tac "ASID (snd (write'mem1 (val, fst (mmu_translate_sat va s), sz) (snd (mmu_translate_sat va s)))) = ASID s \<and>
+                        TTBR0 (snd (write'mem1 (val, fst (mmu_translate_sat va s), sz) (snd (mmu_translate_sat va s)))) = TTBR0 s")
+     apply clarsimp
+    apply (clarsimp simp: snd_def fst_def)
+    apply (case_tac " mmu_translate_sat va s" , clarsimp)
+    apply (case_tac "write'mem1 (val, a, sz) b" , clarsimp)
+    apply (subgoal_tac "ASID b = ASID s \<and> TTBR0 b = TTBR0 s")
+     apply (clarsimp simp: write'mem1_eq_ASID_TTBR0)
+    apply (clarsimp simp: mmu_sat_eq_ASID_TTBR0_MEM)
+   apply (clarsimp simp: snd_def)
+   apply (case_tac " mmu_translate_sat va s" , clarsimp)
+   apply (clarsimp simp: mmu_translate_sat_TLB_union)
+  apply (clarsimp simp: snd_def fst_def)
+  apply (cases "mmu_translate_sat va s" , clarsimp)
+  apply (case_tac "write'mem1 (val, a, sz) b" , clarsimp)
+  apply (clarsimp simp: write'mem1_eq_TLB)
+done
+
+
+lemma
+  "\<lbrakk> saturated t ; consistent t va\<rbrakk> \<Longrightarrow> t = snd (mmu_translate_sat va t)"
+  apply (clarsimp simp: saturated_def mmu_translate_sat_def Let_def split_def)
+  apply (cases "lookup (TLB t \<union> range (pt_walk (ASID t) (MEM t) (TTBR0 t))) (ASID t) (addr_val va)" ; clarsimp)
+    using saturated_not_miss apply blast
+   using sat_con_not_miss_incon sat_state_tlb saturated_def apply auto[1]
+  apply (case_tac "is_fault x3")
+   apply (clarsimp)
+ (* can not do this *)
+  
+
+oops
+
+lemma 
+  "\<lbrakk> write'mem'sat'1 (val,va,sz) s = ((), t); mem1s1 (va, sz) t = (val, r); consistent t va \<rbrakk> 
+                 \<Longrightarrow>  t = r "
+  apply (subgoal_tac "MEM t = MEM r")
+   apply (subgoal_tac "TLB t = TLB r")
+    apply (subgoal_tac "consistent s va")
+     apply (clarsimp simp: write'mem'sat'1_def Let_def split_def)
+     apply (clarsimp simp: mmu_translate_sat_def Let_def)
+     apply (cases " lookup (TLB s \<union> range (pt_walk (ASID s) (MEM s) (TTBR0 s))) (ASID s) (addr_val va)")
+      using saturated_not_miss apply blast
+     prefer 2
+     apply clarsimp
+    
+    apply (subgoal_tac "mmu_translate_sat va t = mmu_translate_sat va r")
+
+
+  apply (clarsimp simp: mem1s1_def Let_def split_def split:split_if_asm)
+
+
+oops
+
+lemma 
+  "\<lbrakk> write'mem'sat'1 (val,va,sz) s = ((), t); mem1s1 (va, sz) t = (val, r); consistent t va \<rbrakk> 
+                 \<Longrightarrow> fst (mmu_translate_sat va s) =  fst (mmu_translate_sat va t)"
+  apply (subgoal_tac "TLB t = TLB s \<union> range (pt_walk (ASID s) (MEM s) (TTBR0 s)) \<or>
+                      TLB t = TLB s \<union> range (pt_walk (ASID s) (MEM s) (TTBR0 s)) \<union> range (pt_walk (ASID t) (MEM t) (TTBR0 t))")
+   prefer 2
+   apply (clarsimp simp: write'mem'sat'1_TLBs)
+  apply (subgoal_tac "saturated t")
+   prefer 2
+   apply (clarsimp simp: write'_not_in_translation_tables_saturated1)
+  apply (subgoal_tac "lookup (TLB s) (ASID s) (addr_val va) \<le> lookup (TLB t) (ASID s) (addr_val va)")
+   apply (clarsimp simp: mmu_translate_sat_def Let_def)
+   apply (cases "lookup (TLB t \<union> range (pt_walk (ASID t) (MEM t) (TTBR0 t))) (ASID t) (addr_val va)")
+     using saturated_not_miss apply blast
+    using sat_con_not_miss_incon sat_state_tlb apply auto[1]
+   apply (case_tac "is_fault x3")
+    apply (erule disjE)
+     apply (clarsimp simp:raise'exception_def)
+   
+
+
+
+
+
+
+
+
+
+
+
+
+
+
+  
+   prefer 2
+proof -
+  assume "TLB t = TLB s \<union> range (pt_walk (ASID s) (MEM s) (TTBR0 s)) \<or> TLB t = TLB s \<union> range (pt_walk (ASID s) (MEM s) (TTBR0 s)) \<union> range (pt_walk (ASID t) (MEM t) (TTBR0 t))"
+  then have "TLB s \<subseteq> TLB t"
+    by blast
+  then show "lookup (TLB s) (ASID s) (addr_val va) \<le> lookup (TLB t) (ASID s) (addr_val va)"
+    by (meson tlb_mono)
+next
+  apply (clarsimp simp: mmu_translate_def)
+ 
+
+   apply (clarsimp simp: tlb_mono)
+  apply (clarsimp simp: write'mem'sat'1_def)
+  apply (cases "mmu_translate_sat va s" , clarsimp)
+  apply (clarsimp simp: mmu_translate_sat_def Let_def)
+  apply (cases "lookup (TLB s \<union> range (pt_walk (ASID s) (MEM s) (TTBR0 s))) (ASID s) (addr_val va)")
+    apply (clarsimp simp: saturated_not_miss)
+   apply (subgoal_tac "TLB s \<union> range (pt_walk (ASID s) (MEM s) (TTBR0 s))
+                             \<union> range (pt_walk (ASID t) (MEM t) (TTBR0 t))= TLB t \<and> ASID s = ASID t")
+    apply (subgoal_tac "lookup (TLB s \<union> range (pt_walk (ASID s) (MEM s) (TTBR0 s))) (ASID s) (addr_val va) \<le> lookup (TLB s \<union> range (pt_walk (ASID s) (MEM s) (TTBR0 s))
+                                      \<union> range (pt_walk (ASID t) (MEM t) (TTBR0 t))) (ASID s) (addr_val va)")
+     apply (clarsimp simp: consistent0_def)
+    apply (clarsimp simp: tlb_mono consistent0_def)
+    apply (metis (no_types, hide_lams) lookup_incon_subset sup.cobounded1)
+   apply (case_tac "write'mem1 (val, a, sz) b" , clarsimp)
+   apply (clarsimp simp: raise'exception_def write'mem1_eq_ASID_TTBR0 write'mem1_eq_TLB split:split_if_asm)
+  apply (clarsimp simp: mem1s1_def)
+  apply (cases "mmu_translate_sat va t" , clarsimp)
+  apply (clarsimp simp: mmu_translate_sat_def Let_def)
+  apply (cases "lookup (TLB t \<union> range (pt_walk (ASID t) (MEM t) (TTBR0 t))) (ASID t) (addr_val va)")
+    apply (clarsimp simp: saturated_not_miss)
+   apply (subgoal_tac "TLB t = TLB t \<union> range (pt_walk (ASID t) (MEM t) (TTBR0 t))")
+    apply (clarsimp simp: consistent0_def)
+   using saturated_def apply blast
+  apply (clarsimp split: split_if_asm)
+      apply (clarsimp simp: raise'exception_def split:split_if_asm)
+  
+  
+ 
+
+
+
+   apply (clarsimp simp: consistent0_def)
+  apply (clarsimp split:split_if_asm)
+    apply ()
+
+
+oops
+
+lemma
+  "\<lbrakk>write'mem1 (val, HOL.undefined, sz) (b\<lparr>exception := PAGE_FAULT ''more info''\<rparr>) = ((), ba) \<rbrakk>   \<Longrightarrow> 
+        (b\<lparr>exception := PAGE_FAULT ''more info''\<rparr>) = ba"
+  apply (clarsimp simp: write'mem1_def split:split_if_asm)
+    apply (clarsimp simp: Let_def)
+
+oops
+
+lemma state:
+  "\<lbrakk> write'mem'sat'1 (val,va,sz) s = ((), t); mem1s (va, sz) t = (val, r); consistent t va \<rbrakk> 
+                 \<Longrightarrow> t = r "
+  apply (clarsimp simp: write'mem'sat'1_def)
+  apply (cases "mmu_translate_sat va s" , clarsimp)
+  apply (clarsimp simp: mmu_translate_sat_def Let_def)
+  apply (cases "lookup (TLB s \<union> range (pt_walk (ASID s) (MEM s) (TTBR0 s))) (ASID s) (addr_val va)")
+    apply (clarsimp simp: saturated_not_miss)
+   apply (subgoal_tac "TLB s \<union> range (pt_walk (ASID s) (MEM s) (TTBR0 s))
+                            \<union> range (pt_walk (ASID t) (MEM t) (TTBR0 t))= TLB t \<and> ASID s = ASID t")
+    apply (subgoal_tac "lookup (TLB s \<union> range (pt_walk (ASID s) (MEM s) (TTBR0 s))) (ASID s) (addr_val va) \<le> lookup (TLB s \<union> range (pt_walk (ASID s) (MEM s) (TTBR0 s))
+                            \<union> range (pt_walk (ASID t) (MEM t) (TTBR0 t))) (ASID s) (addr_val va)")
+     apply (clarsimp simp: consistent0_def)
+    apply (clarsimp simp: tlb_mono consistent0_def)
+    apply (metis (no_types, hide_lams) lookup_incon_subset sup.cobounded1)
+   apply (case_tac "write'mem1 (val, a, sz) b" , clarsimp)
+   apply (clarsimp simp: raise'exception_def write'mem1_eq_ASID_TTBR0 write'mem1_eq_TLB split:split_if_asm)
+  apply (clarsimp split:split_if_asm)
+     apply (clarsimp simp: raise'exception_def split:split_if_asm)
+   apply (case_tac "write'mem1 (val, a, sz) b" , clarsimp)
+   apply (clarsimp simp: raise'exception_def)
+
+
+    apply (clarsimp simp: consistent0_def)
+   apply (case_tac "write'mem1 (val, a, sz) b" , clarsimp)
+   apply (clarsimp simp : write'mem1_eq_ASID_TTBR0 raise'exception_def split:split_if_asm)
+    apply (subgoal_tac "lookup (TLB s) (ASID s) (addr_val va) \<le> lookup (TLB s \<union> range (pt_walk (ASID s) (MEM s) (TTBR0 s))) (ASID s) (addr_val va)")
+     prefer 2
+     apply (simp add: tlb_mono)
+
+
+
+
+
+
+
+
+
+
+
+
+
+
+
+
+
+
+
+
+
+
+(* Redentant Code from here *)
+
+definition 
+  ttbr0_wrp_bit :: "32 word \<Rightarrow> bool"
+where
+  "ttbr0_wrp_bit ttbr0 = hd (to_bl (ucast (ttbr0 AND 0x1) :: 1 word))"
+
+
+definition
+  "write'mem'sat1" :: "bool list \<times> 32 word \<times> nat \<Rightarrow> state \<Rightarrow> unit \<times> state"
+where
+  "write'mem'sat1 \<equiv> \<lambda>(value, vaddr, size). do {
+     (* original TLB before memory translation *)
+     tlb0  <- read_state TLB;
+     paddr <- mmu_translate_sat vaddr;
+     asid  <- read_state ASID;
+     ttbr0 <- read_state TTBR0;
+     (* size is in {1, 2, 4, 8} and will be aligned, so will not cross page boundaries *)
+     case ttbr0_wrp_bit ttbr0 of
+           True \<Rightarrow> do {           (* translation table cant be changed *)
+                    write'mem1 (value, paddr, size);
+                    mem   <- read_state MEM;  (* may be this redundant *)
+                    update_state (\<lambda>s. s\<lparr> MEM := mem \<rparr>)
+                    (* ^^ do i have to do this update explicitly ? *)
+                   }
+         | False \<Rightarrow> do {          (* translation table can be changed *)
+                    write'mem1 (value, paddr, size);
+                    mem   <- read_state MEM;
+                    let all_entries = pt_walk asid mem ttbr0 ` UNIV;
+                    let tlb = tlb0 \<union> all_entries;
+                    update_state (\<lambda>s. s\<lparr> TLB := tlb \<rparr>)
+                   }
+  }"
+
+(* s has to be in saturated state *)
+lemma TLB_same_saturated_wrp:
+  "\<lbrakk>write'mem'sat1 (v,va,sz) s = ((), t) ; ttbr0_wrp_bit (TTBR0 s) ; saturated s \<rbrakk> 
+              \<Longrightarrow> TLB t = TLB s"
+  apply (clarsimp simp: write'mem'sat1_def)
+  apply (cases "mmu_translate_sat va s" , clarsimp)
+  apply (subgoal_tac "TTBR0 s = TTBR0 b \<and> TLB b = TLB t")
+   apply (clarsimp)
+   apply (subgoal_tac "TLB s = TLB b")
+    apply (clarsimp)
+   apply (clarsimp simp: mmu_translate_sat_def Let_def)
+   apply (case_tac "lookup (TLB s \<union> range (pt_walk (ASID s) (MEM s) (TTBR0 b))) (ASID s) va" )
+     apply (frule saturated_lookup_not_miss)
+     apply (frule sat_state_tlb ; clarsimp)
+    apply (clarsimp simp:raise'exception_def split:split_if_asm)
+     apply (frule sat_state_tlb)
+     apply clarsimp
+    apply (frule sat_state_tlb)
+    apply clarsimp
+   apply (frule sat_state_tlb)
+   apply (clarsimp simp: raise'exception_def split:split_if_asm)
+  apply (rule conjI)
+   apply (clarsimp simp: mmu_translate_sat_def Let_def , cases " lookup (TLB s \<union> range (pt_walk (ASID s) (MEM s) (TTBR0 s))) (ASID s) va")
+     apply (frule saturated_lookup_not_miss)
+     apply (frule sat_state_tlb ; clarsimp)
+    apply (clarsimp simp:raise'exception_def split:split_if_asm)
+   apply (clarsimp simp:raise'exception_def split:split_if_asm)
+  apply (subgoal_tac "TTBR0 s = TTBR0 b")
+   apply clarsimp
+   apply (clarsimp simp: write'mem1_def raise'exception_def split:split_if_asm)
+  apply (clarsimp simp: mmu_translate_sat_def Let_def , cases " lookup (TLB s \<union> range (pt_walk (ASID s) (MEM s) (TTBR0 s))) (ASID s) va")
+    apply (frule saturated_lookup_not_miss)
+    apply (frule sat_state_tlb ; clarsimp)
+   apply (clarsimp simp:raise'exception_def split:split_if_asm)+
+done
+
+lemma  write'mem1_tlb_same:
+  "write'mem1 (v, a, sz) b = ((), t) \<Longrightarrow> TLB b = TLB t"
+  apply (clarsimp simp: write'mem1_def raise'exception_def split:split_if_asm)
+done
+
+
+lemma write'mem'sat1_tlb_TLB_sat:
+  "\<lbrakk>write'mem'sat1 (v,va,sz) s = ((), t); ttbr0_wrp_bit (TTBR0 s) \<rbrakk> \<Longrightarrow>
+        TLB t = TLB s \<union> pt_walk (ASID s) (MEM s) (TTBR0 s) ` UNIV  "
+  apply (clarsimp simp: write'mem'sat1_def)
+  apply (cases "mmu_translate_sat va s", clarsimp)
+  apply (subgoal_tac "ttbr0_wrp_bit (TTBR0 b)")
+   apply clarsimp
+   apply (subgoal_tac "TLB b = TLB s \<union> range (pt_walk (ASID s) (MEM s) (TTBR0 s))")
+    apply (clarsimp simp: write'mem1_def raise'exception_def split:split_if_asm)
+   apply (clarsimp simp:mmu_translate_sat_TLB_union)
+  apply (subgoal_tac "TTBR0 b = TTBR0 s")
+   apply (clarsimp simp: ttbr0_wrp_bit_def)
+  apply (clarsimp simp: mmu_translate_sat_def Let_def)
+  apply (cases "lookup (TLB s \<union> range (pt_walk (ASID s) (MEM s) (TTBR0 s))) (ASID s) va")
+    apply (clarsimp simp:raise'exception_def split:split_if_asm)+
+done
+
+lemma
+  "\<lbrakk> TLB b = TLB t ; saturated b ; ASID t = ASID b ; TTBR0 t = TTBR0 b\<rbrakk> \<Longrightarrow> 
+      saturated t"
+  apply (unfold saturated_def) [1]
+  apply simp
+  apply (clarsimp simp: pt_walk_def Let_def)
+
+oops
+
+lemma
+  "write'mem'sat1 (v, va, sz) s = ((), t) \<Longrightarrow> saturated t"
+  apply (clarsimp simp: write'mem'sat1_def)
+  apply (cases "mmu_translate_sat va s", clarsimp)
+  apply (subgoal_tac "saturated b")
+   apply (case_tac "ttbr0_wrp_bit (TTBR0 b)", clarsimp)
+    apply (subgoal_tac "TLB b = TLB t")
+     apply (unfold saturated_def) [1]
+     (*apply ((clarsimp simp: write'mem1_def raise'exception_def split:split_if_asm))*)
+
+oops
+
+
+(* declare [[show_types]] *)
+lemma
+ "\<lbrakk>write'mem'sat1 (v,va,sz) s = ((), t) ; ttbr0_wrp_bit (TTBR0 s);
+    write'mem'sat1 (v,va,sz) t = ((), r)  \<rbrakk> \<Longrightarrow> TLB t = TLB r"
+  apply (subgoal_tac "ttbr0_wrp_bit (TTBR0 t)")
+   apply (subgoal_tac "saturated t")
+    apply (clarsimp simp: TLB_same_saturated_wrp)
+   apply (clarsimp simp: write'mem'sat1_def)
+   apply (cases "mmu_translate_sat va s" , clarsimp)
+   apply (subgoal_tac "ttbr0_wrp_bit (TTBR0 b)")
+    apply clarsimp
+    apply (subgoal_tac "saturated b")
+     apply (subgoal_tac "TLB b = TLB t")
+   (* can't go any further without modifying write'mem1 for wrp bit *)
+
+   apply (unfold saturated_def)
+  apply (frule (1) write'mem'sat1_tlb_TLB_sat)
+  apply (unfold saturated_def)
+  apply (frule mem'write'sat_tlb_asid_ttbr0 ; erule conjE ; clarsimp)
+  using saturated_def apply simp
+   apply ()
+   apply ()
+
+oops
+
+(*find the alignment of translation table *)
+(* find the page table size , multiple levels as well *) 
+(* assumption *)
+definition
+  tt_sz :: "ttbr0 \<Rightarrow> 32 word set"
+where
+  "tt_sz ttbr0 \<equiv> {x . ttbr0 \<le> x \<and> x \<le> (ttbr0 + 10)}"
+
+
+definition
+  "write'mem'sat2" :: "bool list \<times> 32 word \<times> nat \<Rightarrow> state \<Rightarrow> unit \<times> state"
+where
+  "write'mem'sat2 \<equiv> \<lambda>(value, vaddr, size). do {
+     (* original TLB before memory translation *)
+     tlb0  <- read_state TLB;
+     paddr <- mmu_translate_sat vaddr;
+     asid  <- read_state ASID;
+     ttbr0 <- read_state TTBR0;
+     let paddrset = {x. paddr \<le> x \<and> x \<le> (paddr + of_nat size)};
+     (* size is in {1, 2, 4, 8} and will be aligned, so will not cross page boundaries *)
+     if ttbr0_wrp_bit ttbr0 \<and> paddrset \<inter> tt_sz ttbr0 \<noteq> {} then 
+         raise'exception (IMPLEMENTATION_DEFINED ''Page Table is Write Protected'')  
+     else if ttbr0_wrp_bit ttbr0 \<and> paddrset \<inter> tt_sz ttbr0 = {} then 
+          do {           (* translation table cant be changed *)
+               write'mem1 (value, paddr, size);
+               mem   <- read_state MEM;  (* may be this is redundant *)
+               update_state (\<lambda>s. s\<lparr> MEM := mem \<rparr>)
+                    (* ^^ do i have to do this update explicitly ? *)
+     }
+     else if \<not>ttbr0_wrp_bit ttbr0 \<and> paddrset \<inter> tt_sz ttbr0 = {} then 
+          do {           (* translation table cant be changed *)
+               write'mem1 (value, paddr, size);
+               mem   <- read_state MEM;  (* may be this is redundant *)
+               update_state (\<lambda>s. s\<lparr> MEM := mem \<rparr>)
+                    (* ^^ do i have to do this update explicitly ? *)
+     }
+     else 
+          do {          (* translation table can be changed *)
+               write'mem1 (value, paddr, size);
+               mem   <- read_state MEM;
+               let all_entries = pt_walk asid mem ttbr0 ` UNIV;
+               let tlb = tlb0 \<union> all_entries;
+               update_state (\<lambda>s. s\<lparr> TLB := tlb \<rparr>)
+     }
+  }"
+
+
+
+definition
+  write'mem2 :: "bool list \<times> 32 word \<times> nat \<Rightarrow> state \<Rightarrow> unit \<times> state"
+where
+  "write'mem2 \<equiv> 
+   \<lambda>(value, address, size).
+   do {
+   ttbr0 <- read_state TTBR0;
+   if address \<notin> tt_sz ttbr0 then do {
+   if size = 1 then do {
+                      v \<leftarrow> read_state MEM;
+                      v \<leftarrow> return (v(address + 0 := of_bl (bitstring_field 7 0 value)));
+                      update_state (MEM_update (\<lambda>_. v))
+                    }
+   else if size = 2 then do {
+                           do {
+                               v \<leftarrow> read_state MEM;
+                               v \<leftarrow> return (v(address + 0 := of_bl (bitstring_field 7 0 value)));
+                               update_state (MEM_update (\<lambda>_. v))
+                             };
+                           v \<leftarrow> read_state MEM;
+                           v \<leftarrow> return (v(address + 1 := of_bl (bitstring_field 15 8 value)));
+                           update_state (MEM_update (\<lambda>_. v))
+                         }
+        else if size = 4 then do {
+                                do {
+                                    v \<leftarrow> read_state MEM;
+                                    v \<leftarrow> return (v(address + 0 := of_bl (bitstring_field 7 0 value)));
+                                    update_state (MEM_update (\<lambda>_. v))
+                                  };
+                                 do {
+                                    v \<leftarrow> read_state MEM;
+                                    v \<leftarrow> return (v(address + 1 := of_bl (bitstring_field 15 8 value)));
+                                    update_state (MEM_update (\<lambda>_. v))
+                                  };
+                                 do {
+                                    v \<leftarrow> read_state MEM;
+                                    v \<leftarrow> return (v(address + 2 := of_bl (bitstring_field 23 16 value)));
+                                    update_state (MEM_update (\<lambda>_. v))
+                                  };
+                                v \<leftarrow> read_state MEM;
+                                v \<leftarrow> return (v(address + 3 := of_bl (bitstring_field 31 24 value)));
+                                update_state (MEM_update (\<lambda>_. v))
+                              }
+             else if size = 8 then do {
+                                      do {
+                                         v \<leftarrow> read_state MEM;
+                                         v \<leftarrow> return (v(address + 0 := of_bl (bitstring_field 7 0 value)));
+                                         update_state (MEM_update (\<lambda>_. v))
+                                       };
+                                      do {
+                                         v \<leftarrow> read_state MEM;
+                                         v \<leftarrow> return (v(address + 1 := of_bl (bitstring_field 15 8 value)));
+                                         update_state (MEM_update (\<lambda>_. v))
+                                       };
+                                     do {
+                                         v \<leftarrow> read_state MEM;
+                                         v \<leftarrow> return (v(address + 2 := of_bl (bitstring_field 23 16 value)));
+                                         update_state (MEM_update (\<lambda>_. v))
+                                       };
+                                      do {
+                                         v \<leftarrow> read_state MEM;
+                                         v \<leftarrow> return (v(address + 3 := of_bl (bitstring_field 31 24 value)));
+                                         update_state (MEM_update (\<lambda>_. v))
+                                       };
+                                     do {
+                                         v \<leftarrow> read_state MEM;
+                                         v \<leftarrow> return (v(address + 4 := of_bl (bitstring_field 39 32 value)));
+                                         update_state (MEM_update (\<lambda>_. v))
+                                       };
+                                      do {
+                                         v \<leftarrow> read_state MEM;
+                                         v \<leftarrow> return (v(address + 5 := of_bl (bitstring_field 47 40 value)));
+                                         update_state (MEM_update (\<lambda>_. v))
+                                       };
+                                      do {
+                                         v \<leftarrow> read_state MEM;
+                                         v \<leftarrow> return (v(address + 6 := of_bl (bitstring_field 55 48 value)));
+                                         update_state (MEM_update (\<lambda>_. v))
+                                       };
+                                     v \<leftarrow> read_state MEM;
+                                     v \<leftarrow> return (v(address + 7 := of_bl (bitstring_field 63 56 value)));
+                                     update_state (MEM_update (\<lambda>_. v))
+                                   }
+                  else raise'exception (ASSERT ''mem: size in {1, 2, 4, 8}'')  
+   }
+  else  raise'exception (IMPLEMENTATION_DEFINED ''Page Table is Write Protected'')   
+   }"
+
+
+lemma abc:
+  "\<lbrakk>write'mem'sat2 (v,va,sz) s = ((), t) ; ttbr0_wrp_bit (TTBR0 s) ; saturated s \<rbrakk> 
+              \<Longrightarrow> TLB t = TLB s"
+  apply (clarsimp simp: write'mem'sat2_def)
+  apply (cases "mmu_translate_sat va s" , clarsimp)
+  apply (subgoal_tac "ttbr0_wrp_bit (TTBR0 b)")
+   apply (subgoal_tac "TTBR0 s = TTBR0 b \<and> TLB b = TLB t")
+    apply (subgoal_tac "TLB s = TLB b")
+     apply (case_tac "a \<in> tt_sz (TTBR0 b)")
+      apply (clarsimp  simp: raise'exception_def split: split_if_asm)
+     apply (clarsimp)
+    apply (clarsimp simp: mmu_translate_sat_def Let_def)
+    apply (case_tac "lookup (TLB s \<union> range (pt_walk (ASID s) (MEM s) (TTBR0 b))) (ASID s) va" )
+      apply (frule saturated_lookup_not_miss)
+      apply (frule sat_state_tlb ; clarsimp)
+     apply (clarsimp simp: raise'exception_def saturated_def split:split_if_asm)
+    apply (cases s, case_tac b, clarsimp)
+    apply (cases s, cases t, force)
+     apply (cases s, case_tac b, clarsimp)
+     apply (cases s, cases t, force)
+    sorry
+      
+
+
+lemma
+ "\<lbrakk>write'mem'sat2 (v,va,sz) s = ((), t) ; ttbr0_wrp_bit (TTBR0 s);
+    write'mem'sat2 (v,va,sz) t = ((), r)  \<rbrakk> \<Longrightarrow> TLB t = TLB r"
+  apply (subgoal_tac "ttbr0_wrp_bit (TTBR0 t)")
+   apply (subgoal_tac "saturated t")
+    apply (clarsimp simp: abc)
+   apply (clarsimp simp: write'mem'sat2_def)
+   apply (cases "mmu_translate_sat va s" , clarsimp)
+   apply (subgoal_tac "ttbr0_wrp_bit (TTBR0 b)")
+    apply (case_tac "a \<in> tt_sz (TTBR0 b)")
+     apply (clarsimp)
+     apply (subgoal_tac "saturated b")
+      apply (clarsimp simp: raise'exception_def
+      split:split_if_asm)
+      apply (unfold saturated_def) [1]
+      apply simp
+     apply (clarsimp simp:mmu_translate_sat_sat)
+    apply (clarsimp)
+    apply (frule mmu_translate_sat_sat)
+    apply (frule write'mem1_tlb_same)
+    apply (unfold saturated_def) [1]
+
+oops
+
+  apply (cases "mmu_translate_sat va s" , clarsimp)
+  apply (subgoal_tac "ttbr0_wrp_bit (TTBR0 b)")
+   apply (case_tac "a \<in> tt_sz (TTBR0 b)")
+    apply (clarsimp simp: raise'exception_def split:split_if_asm)
+  apply (subgoal_tac "ttbr0_wrp_bit (TTBR0 t)")
+   apply (subgoal_tac "saturated t")
+    apply (clarsimp simp: TLB_same_saturated_wrp)
+   apply (clarsimp simp: write'mem'sat1_def)
+   apply (cases "mmu_translate_sat va s" , clarsimp)
+   apply (subgoal_tac "ttbr0_wrp_bit (TTBR0 b)")
+    apply clarsimp
+    apply (subgoal_tac "saturated b")
+     apply (subgoal_tac "TLB b = TLB t")
+
+
+
+
+
+
+thm write'mem1_def
+
+thm MEM_update_def
+
+(* ask Gerwin how to merge this value *)
+ *)
+
