ROOT
@@ -1,3 +1,0 @@
-session TLB = "HOL-Word" +
-  theories
-    TLB_Refine
