Read_Me.txt
@@ -1,0 +1,32 @@
+Files Information:
+
+ARM_Monadic     - Initial Definitions of ARM Model upto memory write and read functions
+                  Memory operations included:
+                    1) mem1       :: "paddr ⇒ 'a state_scheme ⇒ bool list × 'a state_scheme"
+                    2) mem_read1  :: "paddr × nat ⇒ 'b state_scheme ⇒ bool list × 'b state_scheme"
+                    3) write'mem1 :: "bool list × paddr × nat ⇒ 'b state_scheme ⇒ unit × 'b state_scheme"
+
+
+MMU_Ops         - classes definitions of MMU operations
+
+
+ARM_Monadic_Ops - All of the remaining functions of ARM Model
+                  Status: updated memory operations i.e they operate on virtual address
+                          No errors 
+
+
+MMU_ARM         - Instantiating definitions of MMU operations
+                  MMU Refinement theorems
+
+
+
+
+Sorry-ed Proofs:
+
+No. of Proofs   :  5
+File containing :  MMU_ARM.thy
+Names:             sorry1
+                   sorry2
+                   sorry3
+                   sorry4
+                   sorry5
